Heap.v
@@ -1,0 +1,115 @@
+Require Import Coq.FSets.FMapPositive.
+
+Require Import Rustre.Common.
+
+Set Implicit Arguments.
+
+Inductive memory (A: Type): Type := mk_memory {
+  mm_values : PM.t A;
+  mm_instances : PM.t (memory A)
+}.
+
+Section Operations.
+
+  Variable A B: Type.
+  Implicit Type menv: memory A.
+
+  Definition map (f: A -> B)(m: memory A): memory B. Admitted.
+
+  Definition empty_memory : memory A :=
+    {| mm_values := PM.empty _;
+       mm_instances := PM.empty _ |}.
+
+  Definition mfind_mem x menv := PM.find x menv.(mm_values).
+  Definition mfind_inst x menv := PM.find x menv.(mm_instances).
+
+  Definition madd_mem (id: ident) (v: A) (M: memory A) : memory A :=
+    mk_memory (PM.add id v M.(mm_values))
+              M.(mm_instances).
+
+  Definition madd_obj (id: ident) (M': memory A) (M: memory A) : memory A :=
+    mk_memory M.(mm_values)
+                  (PM.add id M' M.(mm_instances)).
+  
+  Lemma mfind_mem_gss:
+    forall x v M,
+      mfind_mem x (madd_mem x v M) = Some v.
+  Proof.
+    intros x v M.
+    unfold mfind_mem, madd_mem.
+    now apply PM.gss.
+  Qed.
+
+  Lemma mfind_mem_gso:
+    forall x y v M,
+      x <> y
+      -> mfind_mem x (madd_mem y v M) = mfind_mem x M.
+  Proof.
+    intros x y v M.
+    unfold mfind_mem, madd_mem.
+    now apply PM.gso.
+  Qed.
+
+  Lemma mfind_inst_gss:
+    forall x v M,
+      mfind_inst x (madd_obj x v M) = Some v.
+  Proof.
+    intros x v M.
+    unfold mfind_inst, madd_obj.
+    now apply PM.gss.
+  Qed.
+
+  Lemma mfind_inst_gso:
+    forall x y v M,
+      x <> y
+      -> mfind_inst x (madd_obj y v M) = mfind_inst x M.
+  Proof.
+    intros x y v M.
+    unfold mfind_inst, madd_obj.
+    now apply PM.gso.
+  Qed.
+
+  Lemma mfind_mem_add_inst:
+    forall x y omenv menv,
+      mfind_mem x (madd_obj y omenv menv) = mfind_mem x menv.
+  Proof.
+    unfold mfind_mem, madd_obj.
+    reflexivity.
+  Qed.
+  
+(*
+Lemma find_mem_gss:
+  forall y c m, mfind_mem y (madd_mem y c m) = Some c.
+Proof.
+  intros. apply PM.gss.
+Qed.
+
+Lemma find_mem_gso:
+  forall x y c m, x <> y -> find_mem x (add_mem y c m) = find_mem x m.
+Proof.
+  intros. apply PM.gso. assumption.
+Qed.
+
+Lemma find_obj_gss:
+  forall y c m, find_obj y (add_obj y c m) = Some c.
+Proof.
+  intros. apply PM.gss.
+Qed.
+
+Lemma find_obj_gso:
+  forall x y c m, x <> y -> find_obj x (add_obj y c m) = find_obj x m.
+Proof.
+  intros. apply PM.gso. assumption.
+Qed.
+
+Lemma find_mem_add_obj:
+  forall x y omenv menv,
+    find_mem x (add_obj y omenv menv) = find_mem x menv.
+Proof.
+  unfold find_mem, add_obj.
+  reflexivity.
+Qed.
+
+*)
+
+End Operations.
